From40To50/Expr.v
@@ -1,0 +1,334 @@
+From Coq Require Import String NArith ZArith DecimalString List Lia.
+
+From Vyper Require Import Config.
+From Vyper.CheckArith Require Import Builtins.
+From Vyper.L10 Require Import Base.
+From Vyper.L40 Require AST.
+From Vyper.L50 Require AST.
+From Vyper.L50 Require Import Types Expr.
+
+From Vyper.L40Metered Require Import Interpret.
+
+From Vyper.From40To50 Require Import Translate Proto.
+
+Definition LocalVarsAgree {C: VyperConfig} (m: memory) (loc: string_map dynamic_value) (cap: N)
+: Prop
+:= let _ := memory_impl in
+   forall k: N, (k < cap)%N ->
+     map_lookup loc (make_var_name "var" k)
+      =
+     Some (existT _ U256 (yul_uint256 (OpenArray.get m k))).
+
+Lemma local_vars_agree_weaken {C: VyperConfig} {m: memory} {loc: string_map dynamic_value}
+                              {old_cap: N} {new_cap: N}
+                              (Bound: (new_cap <= old_cap)%N)
+                              (Ok: LocalVarsAgree m loc old_cap):
+  LocalVarsAgree m loc new_cap.
+Proof.
+unfold LocalVarsAgree in *.
+intros k KN.
+assert (KO: (k < old_cap)%N) by lia.
+apply (Ok k KO).
+Qed.
+
+Lemma local_vars_agree_weaken_left {C: VyperConfig} {m: memory} {loc: string_map dynamic_value}
+                                   {a b: N}
+                                   (Ok: LocalVarsAgree m loc (N.max a b)):
+  LocalVarsAgree m loc a.
+Proof.
+refine (local_vars_agree_weaken _ Ok).
+lia.
+Qed.
+
+Lemma local_vars_agree_weaken_right {C: VyperConfig} {m: memory} {loc: string_map dynamic_value}
+                                    {a b: N}
+                                    (Ok: LocalVarsAgree m loc (N.max a b)):
+  LocalVarsAgree m loc b.
+Proof.
+refine (local_vars_agree_weaken _ Ok).
+lia.
+Qed.
+
+(* L50 might have no value where L40 sees zero. *)
+Definition ExprResultsAgree {C: VyperConfig}
+                            (e40: expr_result uint256)
+                            (e50: expr_result (list dynamic_value))
+                            (n: N)
+:= match e40, e50 with
+   | ExprAbort a40, ExprAbort a50               =>  a40 = a50
+   | ExprSuccess v40, ExprSuccess nil           =>  Z_of_uint256 v40 = 0%Z /\ n = 0%N
+   | ExprSuccess v40, ExprSuccess (v50 :: nil)  =>  v40 = uint256_of_dynamic_value v50 /\ n = 1%N
+   | _, _ => False
+   end.
+
+Definition ResultsAgree {C: VyperConfig}
+                        (result40: world_state * option (expr_result uint256))
+                        (result50: world_state * option (expr_result (list dynamic_value)))
+                        (n: N)
+:= let '(w40, r40) := result40 in
+   let '(w50, r50) := result50 in
+   w40 = w50
+    /\
+   match r40, r50 with
+   | Some e40, Some e50 => ExprResultsAgree e40 e50 n
+   | None, None => True
+   | _, _ => False
+   end.
+
+Definition ValueListsAgree {C: VyperConfig}
+                           (result40: world_state * option (expr_result (list uint256)))
+                           (result50: world_state * option (expr_result (list dynamic_value)))
+:= let '(w40, r40) := result40 in
+   let '(w50, r50) := result50 in
+   w40 = w50
+    /\
+   match r40, r50 with
+   | Some (ExprAbort a40), Some (ExprAbort a50) =>
+        a40 = a50
+   | Some (ExprSuccess e40), Some (ExprSuccess e50) =>
+        e40 = map uint256_of_dynamic_value e50
+   | None, None => True
+   | _, _ => False
+   end.
+
+
+(* loopinfo:
+      (..., $$offset1, $$offset0)
+ *)
+Definition LoopOffsetsAgree {C: VyperConfig}
+                            (loop_info: list L40.Expr.loop_ctx)
+                            (loc: string_map dynamic_value)
+:= let nesting_depth := length loop_info in
+   forall k: nat,
+     k < nesting_depth
+      ->
+     match nth_error (map L40.Expr.loop_offset loop_info) (nesting_depth - 1 - k) with
+     | None => False
+     | Some x => map_lookup loc (make_var_name "offset" (N.of_nat k)) = Some (existT _ U256 (yul_uint256 x))
+     end.
+
+Definition get_cursor {C: VyperConfig} (loop: L40.Expr.loop_ctx)
+: uint256
+:= uint256_of_Z (Z_of_uint256 (L40.Expr.loop_count loop) - 1 - Z.of_nat (L40.Expr.loop_countdown loop)).
+
+Definition LoopCursorsAgree {C: VyperConfig}
+                           (loop_info: list L40.Expr.loop_ctx)
+                           (loc: string_map dynamic_value)
+:= let nesting_depth := length loop_info in
+   forall k: nat,
+     k < nesting_depth
+      ->
+     match nth_error (map get_cursor loop_info) (nesting_depth - 1 - k) with
+     | None => False
+     | Some x => map_lookup loc (make_var_name "cursor" (N.of_nat k)) = Some (existT _ U256 (yul_uint256 x))
+     end.
+
+Definition ProtosAgree {C: VyperConfig}
+                       (protos: string -> option proto)
+                       (builtins: string -> option L50.Builtins.yul_builtin)
+:= forall name,
+     match protos name, builtins name with
+     | None, None => True
+     | Some p, Some b => p_inputs p = L50.Builtins.b_input_types b 
+                          /\
+                         p_outputs p = L50.Builtins.b_output_types b
+     | _, _ => False
+     end.
+
+(*
+Lemma interpret_translated_expr {C: VyperConfig}
+                                {B: builtin_names_config}
+                                {protos: string_map proto}
+                                {e40: L40.AST.expr}
+                                {e50: L50.AST.expr}
+                                {n: N}
+                                {loop_depth: N}
+                                (Ok: translate_expr protos e40 loop_depth = inr (e50, n))
+                                (call40: forall
+                                              (decl: L40.AST.decl)
+                                              (world: world_state)
+                                              (arg_values: list uint256),
+                                            world_state * option (expr_result uint256))
+                                (call50: forall
+                                              (decl: L50.AST.fun_decl)
+                                              (world: world_state)
+                                              (arg_values: list dynamic_value),
+                                            world_state * option (expr_result (list dynamic_value)))
+                                (CallsOk: forall (decl40: L40.AST.decl)
+                                                 (decl50: L50.AST.fun_decl)
+                                                 (Ok: translate_fun_decl B protos decl40 = inr decl50)
+                                                 (world: world_state)
+                                                 (args40: list uint256)
+                                                 (args50: list dynamic_value)
+                                                 (ArgsOk: args40 = map uint256_of_dynamic_value args50),
+                                             ResultsAgree (call40 decl40 world args40)
+                                                          (call50 decl50 world args50) 1%N)
+                                (decls40: string_map L40.AST.decl)
+                                (decls50: string_map L50.AST.fun_decl)
+                                (DeclsOk: translate_fun_decls B protos decls40 = inr decls50)
+                                (builtins40: string -> option builtin)
+                                (builtins50: string -> option L50.Builtins.yul_builtin)
+                                (BuiltinsSafe: forall x,
+                                                 builtins50 ("$" ++ x)%string = None)
+                                (ProtosOk: ProtosAgree (map_lookup protos) builtins50)
+                                (world: world_state)
+                                (loc40: memory)
+                                (loc50: string_map dynamic_value)
+                                (LocalVarsOk: LocalVarsAgree loc40 loc50 (L40.AST.var_cap_expr e40))
+                                (loop_info: list L40.Expr.loop_ctx)
+                                (LoopDepthOk: length loop_info = N.to_nat loop_depth)
+                                (OffsetsOk: LoopOffsetsAgree loop_info loc50)
+                                (CursorsOk: LoopCursorsAgree loop_info loc50):
+  ResultsAgree
+    (interpret_expr_metered decls40 call40 builtins40 world loc40 loop_info e40)
+    (interpret_expr builtins50 (map_lookup decls50) call50 world loc50 e50) n.
+Proof.
+revert e50 Ok world.
+induction e40 using L40.AST.expr_ind'; intros; cbn in Ok; inversion Ok; subst; cbn; cbn in LocalVarsOk.
+{ (* const *) easy. }
+{ (* local var *)
+  assert (L := LocalVarsOk name (N.lt_succ_diag_r name)).
+  cbn in L. unfold map_lookup in L. now rewrite L.
+}
+{ (* offset *)
+  clear H0.
+  remember (loop_depth =? 0)%N as loop_depth_is_0.
+  destruct loop_depth_is_0. { discriminate. }
+  inversion Ok; subst; cbn; cbn in LocalVarsOk.
+  unfold LoopOffsetsAgree in OffsetsOk.
+  assert (L: length loop_info <> 0).
+  {
+    rewrite LoopDepthOk.
+    intro H.
+    replace 0 with (N.to_nat 0%N) in H by trivial.
+    apply N2Nat.inj in H.
+    subst.
+    discriminate.
+  }
+  assert (J := OffsetsOk (Nat.pred (length loop_info)) (Nat.lt_pred_l _ L)).
+  replace (length loop_info - 1 - Nat.pred (length loop_info)) with 0 in J by lia.
+  destruct loop_info as [|loop]. { contradiction. }
+  cbn in J. unfold map_lookup in J.
+  replace (N.pred loop_depth) with (N.of_nat (length loop_info)) by (cbn in LoopDepthOk; lia).
+  now rewrite J.
+}
+{ (* cursor *) (* dup from offset *)
+  clear H0.
+  remember (loop_depth =? 0)%N as loop_depth_is_0.
+  destruct loop_depth_is_0. { discriminate. }
+  inversion Ok; subst; cbn; cbn in LocalVarsOk.
+  unfold LoopCursorsAgree in CursorsOk.
+  assert (L: length loop_info <> 0).
+  {
+    rewrite LoopDepthOk.
+    intro H.
+    replace 0 with (N.to_nat 0%N) in H by trivial.
+    apply N2Nat.inj in H.
+    subst.
+    discriminate.
+  }
+  assert (J := CursorsOk (Nat.pred (length loop_info)) (Nat.lt_pred_l _ L)).
+  replace (length loop_info - 1 - Nat.pred (length loop_info)) with 0 in J by lia.
+  destruct loop_info as [|loop]. { contradiction. }
+  cbn in J. unfold map_lookup in J.
+  replace (N.pred loop_depth) with (N.of_nat (length loop_info)) by (cbn in LoopDepthOk; lia).
+  now rewrite J.
+}
+{ (* PrivateCall *)
+  assert (F := translate_fun_decls_ok DeclsOk name).
+  remember (fix translate_expr_list (C : VyperConfig) (l : list L40.AST.expr) (loop_depth : N) {struct l} :
+         string + list AST.expr := _) as translate_expr_list.
+  remember (translate_expr_list C args loop_depth) as maybe_args'.
+  destruct maybe_args' as [err | args']. { discriminate. }
+  inversion Ok. subst e50 n. cbn.
+
+  (* looking up the same function in both maps *)
+  cbn in BuiltinsSafe.
+  rewrite BuiltinsSafe.
+  destruct (map_lookup decls40 name) as [d40|].
+  2:{ cbn in F. now destruct (map_lookup decls50). }
+  cbn in F. destruct (map_lookup decls50) as [d50|]. 2:contradiction.
+
+  (* args *)
+  remember (fix interpret_expr_list (world0 : world_state) (loc : memory) (e : list L40.AST.expr):
+              world_state * option (expr_result (list uint256)) := _) as interpret_list_40.
+  remember (fix interpret_expr_list (world0 : world_state) (loc : string_map dynamic_value) (args0 : list AST.expr) :
+              world_state * option (expr_result (list dynamic_value)) := _) as interpret_list_50.
+  assert (V: ValueListsAgree (interpret_list_40 world loc40 args)
+                             (interpret_list_50 world loc50 args')).
+  {
+    symmetry in Heqmaybe_args'.
+    clear Ok H1.
+    revert args' Heqmaybe_args' world H.
+    rewrite Heqtranslate_expr_list.
+    induction args; intros; cbn; cbn in Heqmaybe_args'.
+    { inversion Heqmaybe_args'. now subst. }
+    remember (translate_expr protos a loop_depth) as maybe_a'.
+    destruct maybe_a' as [|(h', n)]. { discriminate. }
+    (* arg must eval to 1 value only *)
+    remember (n =? 1)%N as n_is_1. destruct n_is_1. 2:discriminate.
+    symmetry in Heqn_is_1. apply N.eqb_eq in Heqn_is_1. subst n.
+    rewrite<- Heqtranslate_expr_list in Heqmaybe_args'.
+    remember (translate_expr_list C args loop_depth) as maybe_args_t'.
+    destruct maybe_args_t' as [|t']. { discriminate. }
+    inversion Heqmaybe_args'. subst args'. clear Heqmaybe_args'.
+    rewrite Heqtranslate_expr_list in Heqmaybe_args_t'.
+    assert (TailOk := IHargs (local_vars_agree_weaken_right LocalVarsOk)
+                             t' (eq_sym Heqmaybe_args_t') world
+                             (Forall_inv_tail H)).
+    rewrite Heqinterpret_list_40. cbn. rewrite<- Heqinterpret_list_40.
+    rewrite Heqinterpret_list_50. cbn. rewrite<- Heqinterpret_list_50.
+    destruct (interpret_list_40 world loc40 args) as (world', result40).
+    destruct (interpret_list_50 world loc50 t') as (world50, result50).
+    (* figure out what the arg tail evaluates to *)
+    unfold ValueListsAgree. unfold ValueListsAgree in TailOk.
+    destruct TailOk as (W, R). subst world50.
+    destruct result40 as [result40|]. 2:{ now destruct result50. }
+    destruct result40 as [values40 | abort40].
+    2:{
+      destruct result50 as [result50|]. 2:{ contradiction. }
+      destruct result50 as [values50 | abort50]. { contradiction. }
+      now subst.
+    }
+    destruct result50 as [result50|]. 2:{ contradiction. }
+    destruct result50 as [values50 | abort50]. 2:{ contradiction. }
+    (* arg tail evaluated successfully, let's see what the head does *)
+    assert (HeadOk := Forall_inv H (local_vars_agree_weaken_left LocalVarsOk)
+                                 h' (eq_sym Heqmaybe_a') world').
+    unfold ResultsAgree in HeadOk.
+    destruct (interpret_expr_metered decls40 call40 builtins40 world' loc40 loop_info a) as (w40, r40).
+    destruct (interpret_expr builtins50 (map_lookup decls50) call50 world' loc50 h') as (w50, r50).
+    destruct HeadOk as (W, HeadOk).
+    split. { exact W. }
+    destruct r40 as [r40 |], r50 as [r50 |]; try easy.
+    unfold ExprResultsAgree in HeadOk.
+    destruct r40 as [v40 | a40], r50 as [v50 | a50]; try easy.
+    unfold cons_eval_results.
+    destruct v50. { destruct HeadOk. discriminate. }
+    destruct v50. 2:{ contradiction. }
+    destruct HeadOk as (HeadOk, _).
+    cbn.
+    now f_equal.
+  }
+  (* do the call *)
+  destruct (interpret_list_40 world loc40 args) as (w40, r40).
+  destruct (interpret_list_50 world loc50 args') as (w50, r50).
+  unfold ValueListsAgree in V. destruct V as (W, V).
+  destruct r40 as [[v40|a40] | ], r50 as [[v50|a50] | ]; try easy.
+  subst w50.
+  exact (CallsOk d40 d50 F w40 v40 v50 V).
+}
+(* builtin call *)
+remember (fix translate_expr_list (C : VyperConfig) (l : list L40.AST.expr) (loop_depth : N) {struct l} :
+       string + list AST.expr := _) as translate_expr_list.
+remember (translate_expr_list C args loop_depth) as maybe_args'.
+destruct maybe_args' as [err | args']. { discriminate. }
+remember (Map.lookup protos name) as maybe_proto.
+destruct maybe_proto as [proto|]. 2:discriminate.
+inversion Ok. subst e50 n. cbn.
+remember (fix interpret_expr_list (world0 : world_state) (loc : memory) (e : list L40.AST.expr):
+            world_state * option (expr_result (list uint256)) := _) as interpret_list_40.
+remember (fix interpret_expr_list (world0 : world_state) (loc : string_map dynamic_value) (args0 : list AST.expr) {struct
+                args0} : world_state * option (expr_result (list dynamic_value)) := _) as interpret_list_50.
+assert (P := ProtosOk name). unfold map_lookup in P. rewrite<- Heqmaybe_proto in P.
+*)
