From40To50/Proto.v
@@ -1,0 +1,68 @@
+From Coq Require Import String.
+
+From Vyper.L50 Require Import Types.
+From Vyper Require Import Config ProtoAST.
+
+Local Open Scope list_scope.
+Local Open Scope string_scope.
+
+Record proto := {
+  p_name: string;
+  p_inputs: list yul_type;
+  p_outputs: list yul_type;
+}.
+
+(* We take "address" to mean u256 because Yul has no address type. *)
+Definition read_type (s: string)
+: option yul_type
+:= if string_dec s "address"
+     then Some U256
+     else type_of_string s.
+
+Fixpoint read_types (src: list string)
+: string + list yul_type
+:= match src with
+   | nil => inr nil
+   | h :: t => match read_type h with
+               | None => inl ("unrecognized type: " ++ h)
+               | Some h' => match read_types t with
+                            | inl err => inl err
+                            | inr t' => inr (h' :: t')
+                            end
+               end
+   end.
+
+Definition make_proto (ast: proto_ast)
+: string + proto
+:= match read_types (proto_inputs ast) with
+   | inl err => inl err
+   | inr inputs => 
+      match read_types (proto_outputs ast) with
+      | inl err => inl err
+      | inr outputs => inr {| p_name := proto_name ast
+                            ; p_inputs := inputs
+                            ; p_outputs := outputs
+                           |}
+      end
+   end.
+
+(** The parameter of type [list proto_ast] should be either embedded into the compiler
+    (see builtins.list, haskell/GenerateBuiltinsTable.hs) or should be provided as an
+    external file and parsed via haskell/BuiltinsParser.y).
+ *)
+Definition make_proto_table {C: VyperConfig} (asts: list proto_ast) 
+: string + string_map proto
+:= let _ := string_map_impl in
+   let fix add_protos (l: list proto_ast) (table: string_map proto)
+       : string + string_map proto
+       := match l with
+          | nil => inr table
+          | h :: t => match make_proto h with
+                      | inl err => inl err
+                      | inr p => match Map.lookup table (p_name p) with
+                                 | None => add_protos t (Map.insert table (p_name p) p)
+                                 | _ => inl ("a prototype with that name already exists: " ++ p_name p)
+                                 end
+                      end
+          end
+   in add_protos asts Map.empty.
