From40To50/Translate.v
@@ -1,0 +1,384 @@
+From Coq Require Import String NArith DecimalString List.
+
+From Vyper Require Import Config Range.
+From Vyper.CheckArith Require Import Builtins.
+From Vyper.L10 Require Import Base.
+From Vyper.L40 Require AST.
+From Vyper.L50 Require AST.
+From Vyper.L50 Require Import Types.
+From Vyper.From40To50 Require Import Proto.
+
+Local Open Scope list_scope.
+Local Open Scope string_scope.
+
+Definition make_var_name (id: string) (index: N)
+:= ("$$" ++ id ++ NilZero.string_of_uint (N.to_uint index))%string.
+
+(** Returns the resulting expression and the number of expected values. *)
+Fixpoint translate_expr {C: VyperConfig} (protos: string_map proto)
+                        (e: L40.AST.expr) (loop_depth: N)
+: string + L50.AST.expr * N
+:= let _ := string_map_impl in
+   let fix translate_expr_list {C: VyperConfig} (l: list L40.AST.expr) (loop_depth: N)
+       : string + list L50.AST.expr
+       := match l with
+          | nil => inr nil
+          | cons h t => match translate_expr protos h loop_depth with
+                        | inl err => inl err
+                        | inr (h', n) =>
+                            if (n =? 1)%N
+                              then match translate_expr_list t loop_depth with
+                                   | inl err => inl err
+                                   | inr t' => inr (cons h' t')
+                                   end
+                              else inl "an expression with exactly one value expected in an expr list"
+                        end
+          end
+   in match e with
+      | L40.AST.Const value => inr (L50.AST.Const U256 (yul_uint256 value), 1%N)
+      | L40.AST.LocalVar index => inr (L50.AST.LocVar (make_var_name "var" index), 1%N)
+      | L40.AST.LoopOffset => if (loop_depth =? 0)%N
+                                then inl "LoopOffset outside of a loop"
+                                else inr (L50.AST.LocVar (make_var_name "offset" (N.pred loop_depth)), 1%N)
+      | L40.AST.LoopCursor => if (loop_depth =? 0)%N
+                                then inl "LoopCursor outside of a loop"
+                                else  inr (L50.AST.LocVar (make_var_name "cursor" (N.pred loop_depth)), 1%N)
+      | L40.AST.PrivateCall name args => 
+          match translate_expr_list args loop_depth with
+          | inl err => inl err
+          | inr args' => inr (L50.AST.FunCall ("$" ++ name) args', 1%N)
+          end
+      | L40.AST.BuiltinCall name args =>
+          match translate_expr_list args loop_depth with
+          | inl err => inl err
+          | inr args' =>
+              match Map.lookup protos name with
+              | None => inl ("Unable to find a prototype for a builtin call: " ++ name)
+              | Some p => inr (L50.AST.FunCall name args', N.of_nat (length (p_outputs p)))
+              end
+          end
+      end.
+
+Definition translate_small_stmt {C: VyperConfig}
+                                (protos: string_map proto)
+                                (ss: L40.AST.small_stmt)
+                                (loop_depth: N)
+: string + list L50.AST.stmt
+:= match ss with
+   | L40.AST.Abort AbortBreak    => inr (L50.AST.Break :: nil)
+   | L40.AST.Abort AbortContinue => inr (L50.AST.Continue :: nil)
+   | L40.AST.Abort (AbortException code) =>
+        inr
+        (L50.AST.Expr (L50.AST.FunCall "mstore"
+                             (* addr: *)    (L50.AST.Const U256 (yul_uint256 zero256)
+                             (* value: *) :: L50.AST.Const U256 (yul_uint256 code)
+                                          :: nil))
+         :: L50.AST.Expr (L50.AST.FunCall "revert"
+                            (* addr: *)     (L50.AST.Const U256 (yul_uint256 zero256)
+                            (* len:  *)   :: L50.AST.Const U256 (yul_uint256 one256)
+                                          :: nil))
+         :: nil)
+  | L40.AST.Abort AbortReturnFromContract =>
+        inr (L50.AST.Expr (L50.AST.FunCall "stop" nil) :: nil)
+  | L40.AST.Abort AbortRevert =>
+        inr (L50.AST.Expr (L50.AST.FunCall "revert"
+                                (* addr: *)     (L50.AST.Const U256 (yul_uint256 zero256)
+                                (* len:  *)   :: L50.AST.Const U256 (yul_uint256 zero256)
+                                              :: nil))
+            :: nil)
+  | L40.AST.Return e =>
+        match translate_expr protos e loop_depth with
+        | inl err => inl err
+        | inr (e', 0%N) =>
+                  inr (L50.AST.Expr e'
+                      :: L50.AST.Assign ("$$result" :: nil) (L50.AST.Const U256 (yul_uint256 zero256))
+                      :: L50.AST.Leave
+                      :: nil)
+        | inr (e', 1%N) =>
+                  inr (L50.AST.Assign ("$$result" :: nil) e'
+                      :: L50.AST.Leave
+                      :: nil)
+        | _ => inl "too many values"
+        end
+  | L40.AST.Raise e =>
+        match translate_expr protos e loop_depth with
+        | inl err => inl err
+        | inr (e', 0%N) =>
+            inr (L50.AST.Expr e'
+              :: L50.AST.Expr (L50.AST.FunCall "mstore"
+                                 (* addr: *)     (L50.AST.Const U256 (yul_uint256 zero256)
+                                 (* value: *) :: (L50.AST.Const U256 (yul_uint256 zero256))
+                                              :: nil))
+            :: L50.AST.Expr (L50.AST.FunCall "revert"
+                                (* addr: *)     (L50.AST.Const U256 (yul_uint256 zero256)
+                                (* len:  *)   :: L50.AST.Const U256 (yul_uint256 one256)
+                                              :: nil))
+            :: nil)
+        | inr (e', 1%N) =>
+            inr (L50.AST.Expr (L50.AST.FunCall "mstore"
+                                 (* addr: *)    (L50.AST.Const U256 (yul_uint256 zero256)
+                                 (* value: *) :: e'
+                                              :: nil))
+              :: L50.AST.Expr (L50.AST.FunCall "revert"
+                                  (* addr: *)     (L50.AST.Const U256 (yul_uint256 zero256)
+                                  (* len:  *)   :: L50.AST.Const U256 (yul_uint256 one256)
+                                                :: nil))
+              :: nil)
+        | _ => inl "too many values"
+        end
+  | L40.AST.Assign index e =>
+        match translate_expr protos e loop_depth with
+        | inl err => inl err
+        | inr (e', 0%N) =>
+           inr (L50.AST.Expr e'
+             :: L50.AST.Assign (make_var_name "var" index :: nil) 
+                               (L50.AST.Const U256 (yul_uint256 zero256))
+             :: nil)
+        | inr (e', 1%N) =>
+            inr (L50.AST.Assign (make_var_name "var" index :: nil) e'
+              :: nil)
+        | _ => inl "too many values"
+        end
+  | L40.AST.ExprStmt e =>
+        match translate_expr protos e loop_depth with
+        | inl err => inl err
+        | inr (e', 0%N) => inr (L50.AST.Expr e' :: nil)
+        | inr (e', 1%N) =>
+            inr (L50.AST.Expr (L50.AST.FunCall "pop" (e' :: nil)) :: nil)
+        | _ => inl "too many values"
+        end
+  end.
+
+Fixpoint translate_stmt {C: VyperConfig}
+                        (B: builtin_names_config)
+                        (protos: string_map proto)
+                        (s: L40.AST.stmt)
+                        (loop_depth: N)
+{struct s}
+: string + list L50.AST.stmt
+:= match s with
+   | L40.AST.SmallStmt ss => translate_small_stmt protos ss loop_depth
+   | L40.AST.Switch e cases maybe_default =>
+      let fix translate_cases (l: list L40.AST.case)
+          := match l with
+             | nil => inr nil
+             | (L40.AST.Case guard body) :: t =>
+                  match translate_block B protos body loop_depth with
+                  | inl err => inl err
+                  | inr body' =>
+                      match translate_cases t with
+                      | inl err => inl err
+                      | inr t' => inr (L50.AST.Case U256 (yul_uint256 guard) body' :: t')
+                      end
+                  end
+             end
+      in let translate_default (d: option L40.AST.block)
+             := match d with
+                | None => inr None
+                | Some b => match translate_block B protos b loop_depth with
+                            | inl err => inl err
+                            | inr b' => inr (Some b')
+                            end
+                end
+      in match translate_cases cases with
+         | inl err => inl err
+         | inr cases' =>
+             match translate_default maybe_default with
+             | inl err => inl err
+             | inr default' =>
+                match translate_expr protos e loop_depth with
+                | inl err => inl err
+                | inr (e', 0%N) => inr (L50.AST.Expr e' 
+                                     :: L50.AST.Switch (L50.AST.Const U256 (yul_uint256 zero256))
+                                                       cases' default'
+                                     :: nil)
+                | inr (e', 1%N) => inr (L50.AST.Switch e' cases' default'
+                                     :: nil)
+                | _ => inl "too many values"
+                end
+             end
+         end
+   | L40.AST.Loop index count body =>
+      match translate_block B protos body (N.succ loop_depth) with
+      | inl err => inl err
+      | inr body' =>
+          let offset_var := make_var_name "offset" loop_depth in
+          let cursor_var := make_var_name "cursor" loop_depth in
+          inr (L50.AST.For
+                (L50.AST.Block
+                   (L50.AST.VarDecl ((U256, offset_var) :: nil)
+                                    (Some (L50.AST.LocVar (make_var_name "var" index)))
+                    :: L50.AST.VarDecl ((U256, cursor_var) :: nil) None
+                    :: nil))
+                (L50.AST.FunCall (builtin_name_uint256_lt B)
+                   (L50.AST.LocVar cursor_var 
+                    :: L50.AST.Const U256 (yul_uint256 count)
+                    :: nil))
+                (L50.AST.Block
+                   (L50.AST.Assign (cursor_var :: nil)
+                      (L50.AST.FunCall (builtin_name_uint256_add B)
+                         (L50.AST.LocVar cursor_var 
+                          :: L50.AST.Const U256 (yul_uint256 one256)
+                          :: nil))
+                   :: nil))
+                body'
+              :: nil)
+      end
+   end
+with translate_block {C: VyperConfig}
+                     (B: builtin_names_config)
+                     (protos: string_map proto)
+                     (b: L40.AST.block)
+                     (loop_depth: N)
+: string + L50.AST.block
+:= let '(L40.AST.Block body) := b in
+   let fix translate_stmt_list (l: list L40.AST.stmt)
+       := match l with
+          | nil => inr nil
+          | h :: t => match translate_stmt B protos h loop_depth with
+                      | inl err => inl err
+                      | inr h' => match translate_stmt_list t with
+                                  | inl err => inl err
+                                  | inr t' => inr (h' ++ t')%list
+                                  end
+                      end
+          end
+   in match translate_stmt_list body with
+      | inl err => inl err
+      | inr body' => inr (L50.AST.Block body')
+      end.
+
+Definition make_input_typenames (count: N)
+:= List.map (fun n => (U256, make_var_name "var" n)) (range 0 count).
+
+Definition make_var_declarations {C: VyperConfig} (start finish: N)
+:= map (fun n => L50.AST.VarDecl ((U256, make_var_name "var" n) :: nil) None)
+       (range start (finish - start)%N).
+
+Definition translate_fun_decl {C: VyperConfig}
+                              (B: builtin_names_config)
+                              (protos: string_map proto)
+                              (d: L40.AST.decl)
+: string + L50.AST.fun_decl
+:= let '(L40.AST.FunDecl name args_count body) := d in
+   match translate_block B protos body 0%N with
+   | inl err => inl err
+   | inr (L50.AST.Block body') =>
+      inr {| L50.AST.fd_name := name
+           ; L50.AST.fd_inputs := make_input_typenames args_count
+           ; L50.AST.fd_outputs := (U256, "$$result") :: nil
+           ; L50.AST.fd_body :=
+                L50.AST.Block (make_var_declarations args_count (L40.AST.var_cap_block body) ++ body')
+          |}
+   end.
+
+(* This is a version of alist_maybe_map but we want to map keys too. *)
+Fixpoint alist_maybe_map_kv {Key Value Value' Err: Type}
+                            (KeyEqDec: forall x y: Key, {x = y} + {x <> y})
+                            (a: list (Key * Value))
+                            (fkey: Key -> Key)
+                            (fval: Value -> Err + Value')
+{struct a}
+: Err + list (Key * Value')
+:= match a with
+   | nil => inr nil
+   | cons (k, v) t =>
+      match fval v with
+      | inl err => inl err
+      | inr fv =>
+          match alist_maybe_map_kv KeyEqDec t fkey fval with
+          | inl err => inl err
+          | inr mt => inr (cons (fkey k, fv) mt)
+          end
+      end
+   end.
+
+Lemma alist_maybe_map_kv_ok {Key Value Value' Err: Type}
+                            {KeyEqDec: forall x y: Key, {x = y} + {x <> y}}
+                            {a: list (Key * Value)}
+                            {a': list (Key * Value')}
+                            (fkey: Key -> Key)
+                            {fval: Value -> Err + Value'}
+                            (E: alist_maybe_map_kv KeyEqDec a fkey fval = inr a')
+                            (Inj: forall a b, fkey a = fkey b -> a = b)
+                            (key: Key):
+  match Map.alist_lookup KeyEqDec a key with
+  | Some v =>
+      match fval v with
+      | inl _ => False
+      | inr fv => Map.alist_lookup KeyEqDec a' (fkey key) = Some fv
+      end
+  | None => Map.alist_lookup KeyEqDec a' (fkey key) =None
+  end.
+Proof.
+revert a' E.
+induction a as [|(k, v)]; intros. { cbn in *. inversion E. now subst. }
+cbn in *.
+remember (KeyEqDec key k) as key_k.
+destruct key_k.
+{
+  destruct (fval v). { discriminate. }
+  subst.
+  destruct alist_maybe_map_kv. { discriminate. }
+  inversion E. subst. cbn.
+  now destruct (KeyEqDec (fkey k) (fkey k)).
+}
+destruct (fval v). { discriminate. }
+subst.
+destruct alist_maybe_map_kv. { discriminate. }
+inversion E. subst. cbn.
+destruct (KeyEqDec (fkey key) (fkey k)) as [Ekey|Nkey].
+{ apply Inj in Ekey. contradiction. }
+now apply IHa.
+Qed.
+
+Lemma dollar_inj (a b: string)
+                 (H: ("$" ++ a)%string = ("$" ++ b)%string):
+  a = b.
+Proof.
+now inversion H.
+Qed.
+
+Definition translate_fun_decls {C: VyperConfig}
+                               (B: builtin_names_config)
+                               (protos: string_map proto)
+                               (decls: string_map L40.AST.decl)
+: string + string_map L50.AST.fun_decl
+:= let _ := string_map_impl in 
+   match alist_maybe_map_kv string_dec (Map.items decls)
+                            (fun x => "$" ++ x)%string
+                            (translate_fun_decl B protos)
+   with
+   | inl err => inl err
+   | inr a => inr (Map.of_alist a)
+   end.
+
+Lemma translate_fun_decls_ok {C: VyperConfig}
+                             {B: builtin_names_config}
+                             {protos: string_map proto}
+                             {decls40: string_map L40.AST.decl}
+                             {decls50: string_map L50.AST.fun_decl}
+                             (Ok: translate_fun_decls B protos decls40 = inr decls50)
+                             (name: string):
+  match map_lookup decls40 name, map_lookup decls50 ("$" ++ name)%string with
+  | Some d40, Some d50 => translate_fun_decl B protos d40 = inr d50
+  | None, None => True
+  | _, _ => False
+  end.
+Proof.
+unfold translate_fun_decls in Ok.
+unfold map_lookup in *.
+rewrite Map.items_ok.
+remember (alist_maybe_map_kv _ _ _ _) as a.
+destruct a. { discriminate. }
+inversion Ok. subst decls50. clear Ok.
+symmetry in Heqa. assert (A := alist_maybe_map_kv_ok _ Heqa dollar_inj name).
+destruct (Map.alist_lookup string_dec (Map.items decls40) name); rewrite Map.of_alist_ok.
+{
+  remember (Map.alist_lookup string_dec l name) as x.
+  remember (translate_fun_decl B protos d) as d'.
+  destruct d'. { contradiction. }
+  subst. rewrite A. trivial.
+}
+now rewrite A.
+Qed.
