L40Metered/Stmt.v
@@ -1,0 +1,330 @@
+From Coq Require Import String Arith ZArith PropExtensionality.
+
+From Vyper Require Import Config Calldag.
+From Vyper.L10 Require Import Base.
+From Vyper.L40 Require Import AST Descend Callset Descend Expr Stmt.
+From Vyper.L40Metered Require Import Interpret Expr.
+
+Lemma small_stmt_metering_ok
+           {C: VyperConfig}
+           {bigger_call_depth_bound smaller_call_depth_bound: nat}
+           (Ebound: bigger_call_depth_bound = S smaller_call_depth_bound)
+           {cd: calldag}
+           (fc: fun_ctx cd bigger_call_depth_bound)
+           (do_call: forall
+                         (fc': fun_ctx cd smaller_call_depth_bound)
+                         (world: world_state)
+                         (arg_values: list uint256),
+                       world_state * expr_result uint256)
+           (do_call_metered: forall
+                               (decl: L40.AST.decl)
+                               (world: world_state)
+                               (arg_values: list uint256),
+                             world_state * option (expr_result uint256))
+           (DoCallOk: forall (fc': fun_ctx cd smaller_call_depth_bound)
+                             (world: world_state)
+                             (arg_values: list uint256),
+                        let '(world', result) := do_call fc' world arg_values in
+                          do_call_metered (fun_decl fc') world arg_values
+                           =
+                          (world', Some result))
+           (builtins: string -> option builtin)
+           (world: world_state)
+           (loc: memory)
+           (loops: list loop_ctx)
+           (ss: small_stmt)
+           (CallOk: let _ := string_set_impl in 
+                      FSet.is_subset (small_stmt_callset ss)
+                                     (decl_callset (fun_decl fc))
+                      = true):
+  let '(world', result) := interpret_small_stmt Ebound fc do_call builtins
+                                                world loc loops ss CallOk
+   in interpret_small_stmt_metered (cd_decls cd) do_call_metered builtins
+                                   world loc loops ss
+       =
+      (world', Some result).
+Proof.
+destruct ss.
+{ (* abort *) easy. }
+{ (* return *)
+  cbn.
+  assert (M := expr_metering_ok Ebound fc do_call do_call_metered DoCallOk
+                                builtins world loc loops e
+                                (callset_descend_return eq_refl CallOk)).
+  destruct interpret_expr as (world', result).
+  rewrite M.
+  now destruct result.
+}
+{ (* raise *)
+  cbn.
+  assert (M := expr_metering_ok Ebound fc do_call do_call_metered DoCallOk
+                                builtins world loc loops e
+                                (callset_descend_raise eq_refl CallOk)).
+  destruct interpret_expr as (world', result).
+  rewrite M.
+  now destruct result.
+}
+{ (* assign *)
+  cbn.
+  assert (M := expr_metering_ok Ebound fc do_call do_call_metered DoCallOk
+                                builtins world loc loops rhs
+                                (callset_descend_assign_rhs eq_refl CallOk)).
+  destruct interpret_expr as (world', result).
+  rewrite M.
+  now destruct result.
+}
+(* ExprStmt *)
+cbn.
+assert (M := expr_metering_ok Ebound fc do_call do_call_metered DoCallOk
+                              builtins world loc loops e
+                              (callset_descend_expr_stmt eq_refl CallOk)).
+destruct interpret_expr as (world', result).
+rewrite M.
+now destruct result.
+Qed.
+
+Local Lemma weak_block_metering_ok
+           {C: VyperConfig}
+           {bigger_call_depth_bound smaller_call_depth_bound: nat}
+           (Ebound: bigger_call_depth_bound = S smaller_call_depth_bound)
+           {cd: calldag}
+           (fc: fun_ctx cd bigger_call_depth_bound)
+           (do_call: forall
+                         (fc': fun_ctx cd smaller_call_depth_bound)
+                         (world: world_state)
+                         (arg_values: list uint256),
+                       world_state * expr_result uint256)
+           (do_call_metered: forall
+                               (decl: L40.AST.decl)
+                               (world: world_state)
+                               (arg_values: list uint256),
+                             world_state * option (expr_result uint256))
+           (DoCallOk: forall (fc': fun_ctx cd smaller_call_depth_bound)
+                             (world: world_state)
+                             (arg_values: list uint256),
+                        let '(world', result) := do_call fc' world arg_values in
+                          do_call_metered (fun_decl fc') world arg_values
+                           =
+                          (world', Some result))
+           (builtins: string -> option builtin)
+           (b: block)
+           (StmtOk: (* this condition is what makes this lemma weak,
+                       later we can prove a stronger lemma without this *)
+              match b with
+              | Block body =>
+                 List.Forall
+                   (fun s : stmt =>
+                    forall (CallOk : FSet.is_subset (stmt_callset s) (decl_callset (fun_decl fc)) = true) 
+                      (world : world_state) (loc : memory) (loops : list loop_ctx),
+                    let '(world', result) := interpret_stmt Ebound fc do_call builtins
+                                                            world loc loops s CallOk
+                    in
+                     interpret_stmt_metered (cd_decls cd) do_call_metered builtins
+                                                           world loc loops s 
+                      =
+                    (world', Some result))
+                   body
+              end)
+           (world: world_state)
+           (loc: memory)
+           (loops: list loop_ctx)
+           (CallOk: let _ := string_set_impl in 
+                      FSet.is_subset (block_callset b)
+                                     (decl_callset (fun_decl fc))
+                      = true):
+  let '(world', result) := interpret_block Ebound fc do_call builtins
+                                           world loc loops b CallOk
+   in interpret_block_metered (cd_decls cd) do_call_metered builtins
+                              world loc loops b
+       =
+      (world', Some result).
+Proof.
+destruct b as [body]. cbn.
+remember (callset_descend_block eq_refl CallOk) as COk. clear HeqCOk CallOk.
+revert world loc COk. induction body. { easy. }
+intros. cbn.
+assert (HeadOk := List.Forall_inv StmtOk (callset_descend_stmts_head eq_refl COk)
+                                  world loc loops).
+cbn in HeadOk.
+fold (interpret_stmt Ebound fc do_call builtins world loc loops a).
+destruct interpret_stmt as ((world', loc'), result).
+rewrite HeadOk.
+destruct result; trivial.
+apply (IHbody (List.Forall_inv_tail StmtOk) world' loc'
+              (callset_descend_stmts_tail eq_refl COk)).
+Qed.
+
+Lemma stmt_metering_ok
+           {C: VyperConfig}
+           {bigger_call_depth_bound smaller_call_depth_bound: nat}
+           (Ebound: bigger_call_depth_bound = S smaller_call_depth_bound)
+           {cd: calldag}
+           (fc: fun_ctx cd bigger_call_depth_bound)
+           (do_call: forall
+                         (fc': fun_ctx cd smaller_call_depth_bound)
+                         (world: world_state)
+                         (arg_values: list uint256),
+                       world_state * expr_result uint256)
+           (do_call_metered: forall
+                               (decl: L40.AST.decl)
+                               (world: world_state)
+                               (arg_values: list uint256),
+                             world_state * option (expr_result uint256))
+           (DoCallOk: forall (fc': fun_ctx cd smaller_call_depth_bound)
+                             (world: world_state)
+                             (arg_values: list uint256),
+                        let '(world', result) := do_call fc' world arg_values in
+                          do_call_metered (fun_decl fc') world arg_values
+                           =
+                          (world', Some result))
+           (builtins: string -> option builtin)
+           (world: world_state)
+           (loc: memory)
+           (loops: list loop_ctx)
+           (s: stmt)
+           (CallOk: let _ := string_set_impl in 
+                      FSet.is_subset (stmt_callset s)
+                                     (decl_callset (fun_decl fc))
+                      = true):
+  let '(world', result) := interpret_stmt Ebound fc do_call builtins
+                                                world loc loops s CallOk
+   in interpret_stmt_metered (cd_decls cd) do_call_metered builtins
+                                   world loc loops s
+       =
+      (world', Some result).
+Proof.
+revert world loc loops.
+induction s using stmt_ind'; intros.
+{ (* small *)
+  apply small_stmt_metering_ok.
+  apply DoCallOk.
+}
+{ (* switch without default *)
+  cbn.
+  assert (M := expr_metering_ok Ebound fc do_call do_call_metered DoCallOk
+                                builtins world loc loops e
+                                (callset_descend_switch_expr eq_refl CallOk)).
+  destruct interpret_expr as (world', result).
+  rewrite M. clear M.
+  destruct result as [value|]. 2:reflexivity.
+  remember (callset_descend_cases eq_refl CallOk) as COk. clear HeqCOk CallOk.
+  cbn in COk. revert COk.
+  induction cases as [|h]. { easy. }
+  intro COk.
+  destruct h as [h_guard].
+  fold (interpret_block Ebound fc do_call builtins).
+  destruct (Z_of_uint256 value =? Z_of_uint256 h_guard)%Z.
+  { (* match found *)
+    assert (Hh := List.Forall_inv H). cbn in Hh.
+    apply (weak_block_metering_ok Ebound fc do_call do_call_metered DoCallOk
+                                         builtins body Hh world loc loops
+                                         (callset_descend_cases_head eq_refl COk)).
+  }
+  (* no match *)
+  apply (IHcases (List.Forall_inv_tail H) (callset_descend_cases_tail eq_refl COk)).
+}
+{
+  (* switch with default *)
+  cbn.
+  assert (M := expr_metering_ok Ebound fc do_call do_call_metered DoCallOk
+                                builtins world loc loops e
+                                (callset_descend_switch_expr eq_refl CallOk)).
+  destruct interpret_expr as (world', result).
+  rewrite M. clear M.
+  destruct result as [value|]. 2:reflexivity.
+  remember (callset_descend_cases eq_refl CallOk) as COk. clear HeqCOk.
+  remember (callset_descend_cases_default eq_refl CallOk) as DOk. clear HeqDOk CallOk.
+  cbn in COk. revert COk.
+  induction cases as [|h].
+  {
+    intro Foo.
+    apply (weak_block_metering_ok Ebound fc do_call do_call_metered DoCallOk
+                                  builtins (Block default) H0 world loc loops
+                                  DOk).
+  }
+  intro COk.
+  destruct h as [h_guard].
+  fold (interpret_block Ebound fc do_call builtins).
+  destruct (Z_of_uint256 value =? Z_of_uint256 h_guard)%Z.
+  { (* match found *)
+    assert (Hh := List.Forall_inv H). cbn in Hh.
+    apply (weak_block_metering_ok Ebound fc do_call do_call_metered DoCallOk
+                                         builtins body Hh world loc loops
+                                         (callset_descend_cases_head eq_refl COk)).
+  }
+  (* no match *)
+  apply (IHcases (List.Forall_inv_tail H) (callset_descend_cases_tail eq_refl COk)).
+}
+(* loop *)
+remember (Block body) as loop_body.
+cbn. fold (interpret_block Ebound fc do_call builtins).
+subst loop_body.
+remember (Z.to_nat (Z_of_uint256 count)) as n. clear Heqn.
+remember (OpenArray.get loc var) as offset. clear Heqoffset.
+revert world loc.
+induction n. { trivial. }
+intros.
+assert (W := let _ := memory_impl in
+             weak_block_metering_ok Ebound fc do_call do_call_metered DoCallOk
+                                    builtins (Block body) H world loc
+                                    ({|
+                                       loop_offset := offset;
+                                       loop_count := count;
+                                       loop_countdown := n
+                                    |} :: loops)
+                                    (callset_descend_loop_body eq_refl CallOk)).
+destruct interpret_block as ((world', loc'), result). rewrite W. clear W.
+destruct result. 3:trivial.
+{ apply IHn. }
+destruct a; trivial.
+apply IHn.
+Qed.
+
+Lemma block_metering_ok
+           {C: VyperConfig}
+           {bigger_call_depth_bound smaller_call_depth_bound: nat}
+           (Ebound: bigger_call_depth_bound = S smaller_call_depth_bound)
+           {cd: calldag}
+           (fc: fun_ctx cd bigger_call_depth_bound)
+           (do_call: forall
+                         (fc': fun_ctx cd smaller_call_depth_bound)
+                         (world: world_state)
+                         (arg_values: list uint256),
+                       world_state * expr_result uint256)
+           (do_call_metered: forall
+                               (decl: L40.AST.decl)
+                               (world: world_state)
+                               (arg_values: list uint256),
+                             world_state * option (expr_result uint256))
+           (DoCallOk: forall (fc': fun_ctx cd smaller_call_depth_bound)
+                             (world: world_state)
+                             (arg_values: list uint256),
+                        let '(world', result) := do_call fc' world arg_values in
+                          do_call_metered (fun_decl fc') world arg_values
+                           =
+                          (world', Some result))
+           (builtins: string -> option builtin)
+           (world: world_state)
+           (loc: memory)
+           (loops: list loop_ctx)
+           (b: block)
+           (CallOk: let _ := string_set_impl in 
+                      FSet.is_subset (block_callset b)
+                                     (decl_callset (fun_decl fc))
+                      = true):
+  let '(world', result) := interpret_block Ebound fc do_call builtins
+                                           world loc loops b CallOk
+   in interpret_block_metered (cd_decls cd) do_call_metered builtins
+                              world loc loops b
+       =
+      (world', Some result).
+Proof.
+refine (weak_block_metering_ok Ebound fc do_call do_call_metered DoCallOk
+                               builtins b _ world loc loops CallOk).
+clear CallOk world loc loops.
+destruct b as [body].
+rewrite List.Forall_forall.
+intros s H CallOk world loc loops. clear H.
+apply (stmt_metering_ok Ebound fc do_call do_call_metered DoCallOk
+                        builtins world loc loops).
+Qed.
