L50/AST.v
@@ -1,0 +1,51 @@
+From Coq Require Import String.
+From Vyper Require Import Config.
+From Vyper.L50 Require Import Types.
+
+Inductive expr {C: VyperConfig}
+:= FunCall (name: string) (args: list expr) 
+ | LocVar (name: string)
+ | Const (t: yul_type) (val: yul_value t).
+
+Definition typename: Type := yul_type * string.
+
+Inductive stmt {C: VyperConfig}
+:= BlockStmt (s: block)
+ | VarDecl (vars: list typename) (init: option expr)
+ | Assign (lhs: list string) (rhs: expr)
+ | If (cond: expr) (body: block)
+ | Expr (e: expr)
+ | Switch (e: expr) (cases: list case) (default: option block)
+ | For (init: block) (cond: expr) (after body: block)
+ | Break
+ | Continue
+ | Leave
+with case  {C: VyperConfig} := Case (t: yul_type) (val: yul_value t) (body: block)
+with block {C: VyperConfig} := Block (body: list stmt).
+
+Record fun_decl {C: VyperConfig} := {
+  fd_name: string;
+  fd_inputs: list typename;
+  fd_outputs: list typename;
+  fd_body: block;
+}.
+
+Definition program {C: VyperConfig}: Type := string_map fun_decl * block.
+
+
+Definition is_var_decl {C: VyperConfig} (s: stmt)
+:= match s with
+   | VarDecl _ _ => true
+   | _ => false
+   end.
+
+Program Definition var_decl_unpack {C: VyperConfig} (s: stmt) (IsVarDecl: is_var_decl s = true)
+: list typename * option expr
+:= match s with
+   | VarDecl vars init => (vars, init)
+   | _ => False_rect _ _
+   end.
+Next Obligation.
+destruct s; cbn in IsVarDecl; try discriminate.
+exact (H vars init eq_refl).
+Qed.
