L50/Builtins.v
@@ -1,0 +1,81 @@
+(* Yul's builtins are different from L10-L40 builtins because of the different type system. *)
+
+From Coq Require Import List String Arith.
+
+From Vyper Require Import Config Map NaryFun.
+From Vyper.L10 Require Import Base.
+From Vyper.L50 Require Import Types.
+
+Record yul_builtin {C: VyperConfig} := {
+  b_input_types: list yul_type;
+  b_output_types: list yul_type;
+  b_fun: world_state -> nary_fun uint256 (List.length b_input_types) (world_state * list uint256)
+}.
+
+Fixpoint mass_typecheck {C: VyperConfig} (values: list dynamic_value) (types: list yul_type)
+: bool
+:= match values, types with
+   | nil, nil => true
+   | (existT _ t _) :: vtail, thead :: ttail =>
+      if yul_type_eq_dec t thead
+        then mass_typecheck vtail ttail
+        else false
+   | _, _ => false
+   end.
+
+(* mass typecheck fails if the numbers of values and types mismatch *)
+Lemma mass_typecheck_length {C: VyperConfig} (values: list dynamic_value) (types: list yul_type)
+                            (H: mass_typecheck values types = true):
+  List.length values = List.length types.
+Proof.
+revert types H.
+induction values as [|vhead]; intros; cbn in H; destruct types as [|thead]; try discriminate.
+{ trivial. }
+{ now destruct vhead. }
+cbn. f_equal.
+apply IHvalues.
+destruct vhead as (t, _).
+now destruct (yul_type_eq_dec t thead).
+Qed.
+
+Fixpoint mass_cast {C: VyperConfig} (values: list uint256) (types: list yul_type)
+: string + list dynamic_value
+:= match values, types with
+   | nil, nil => inr nil
+   | vhead :: vtail, thead :: ttail =>
+      match yul_value_of_uint256 vhead thead with
+      | Some v =>
+          match mass_cast vtail ttail with
+          | inl err => inl err
+          | inr tail => inr (existT _ thead v :: tail)
+          end
+      | None => inl ("cannot cast to " ++ string_of_type thead)%string
+      end
+   | _, _ => inl "cannot cast: different number of types"%string
+   end.
+
+Local Lemma call_builtin_helper {C: VyperConfig}
+                                (b: yul_builtin)
+                                (args: list dynamic_value)
+                                (E: mass_typecheck args (b_input_types b) = true):
+  List.length (b_input_types b) <= List.length (List.map uint256_of_dynamic_value args).
+Proof.
+rewrite List.map_length.
+apply Nat.eq_le_incl.
+symmetry.
+apply mass_typecheck_length.
+assumption.
+Qed.
+
+Definition call_builtin {C: VyperConfig} (b: yul_builtin) (world: world_state) (args: list dynamic_value)
+: world_state * expr_result (list dynamic_value)
+:= (if mass_typecheck args (b_input_types b) as a return _ = a -> _
+     then fun E =>
+          let args_u256 := List.map uint256_of_dynamic_value args in
+          let '((world', outputs_256), _) := nary_call (b_fun b world) args_u256
+                                                       (call_builtin_helper b args E)
+           in (world', match mass_cast outputs_256 (b_output_types b) with
+                       | inl err => expr_error err
+                       | inr outputs => ExprSuccess outputs
+                       end)
+     else fun _ => (world, expr_error "builtin argument type mismatch"%string)) eq_refl.
