L50/Call.v
@@ -1,0 +1,46 @@
+From Coq Require Import String Arith ZArith.
+
+From Vyper Require Import Config Map.
+From Vyper.L10 Require Import Base.
+From Vyper.L50 Require Import Types AST Builtins Expr LocalVars DynError Stmt.
+
+
+
+Fixpoint interpret_call {C: VyperConfig}
+                        (max_call_depth: nat)
+                        (max_loop_iterations: nat)
+                        (builtins: string -> option yul_builtin)
+                        (funs: string -> option fun_decl)
+                        (f: fun_decl)
+                        (world: world_state)
+                        (arg_values: list dynamic_value)
+{struct max_call_depth}
+: world_state * option (expr_result (list dynamic_value))
+:= let _ := string_map_impl in
+   match max_call_depth with
+   | O => (world, None)
+   | S new_max_call_depth =>
+        match bind_vars_to_values (fd_inputs f) arg_values Map.empty with
+        | inl err => (world, Some (expr_error (string_of_dynamic_error err)))
+        | inr loc_with_args_only =>
+            match bind_vars_to_zeros (fd_outputs f) loc_with_args_only with
+            | inl err => (world, Some (expr_error (string_of_dynamic_error err)))
+            | inr loc =>
+                let '(world', loc', result) :=
+                        interpret_block max_loop_iterations builtins funs (Some f)
+                                        (interpret_call new_max_call_depth max_loop_iterations 
+                                                        builtins funs)
+                                        world loc nop (fd_body f)
+                in (world', match result with
+                            | None => None
+                            | Some StmtSuccess =>
+                                match get_vars_by_typenames (fd_outputs f) loc with
+                                | inl err => Some (expr_error (string_of_dynamic_error err))
+                                | inr outputs => Some (ExprSuccess outputs)
+                                end
+                            | Some (StmtAbort a) => Some (ExprAbort a)
+                            | Some (StmtReturnFromFunction x) => Some (ExprSuccess x)
+                            end)
+            end
+        end
+   end.
