L50/DynError.v
@@ -1,0 +1,67 @@
+From Coq Require Import String.
+
+From Vyper Require Import Config Map.
+From Vyper.L10 Require Import Base.
+From Vyper.L50 Require Import Types.
+
+Local Open Scope string_scope.
+
+(**
+  An error that can occur during dynamic evaluation.
+  This only includes errors that become impossible with static typing.
+ *)
+Inductive dynamic_error
+:= DE_CannotResolveLocalVariable (name: string)
+ | DE_TypeMismatch (expected actual: yul_type)
+
+   (** A function is called with extra arguments
+    or a variable declaration with an initializer has too few variables. *)
+ | DE_TooManyValues
+
+   (** A function is called with not enough arguments
+    or an variable declaration with an initializer has too many variables. *)
+ | DE_TooFewValues
+ | DE_LocalNameShadowing (name: string)
+ | DE_LeaveWithoutFunction
+ | DE_LeftoverValuesInExpression
+ | DE_SingleBooleanExpected
+ | DE_SingleValueExpected
+ | DE_BreakContinueDisallowed.
+
+Definition string_of_dynamic_error (d: dynamic_error)
+:= match d with
+   | DE_CannotResolveLocalVariable name => "cannot resolve local variable: " ++ name
+   | DE_TypeMismatch expected actual => "type mismatch, expected: " ++ string_of_type expected ++
+                                        ", got: " ++ string_of_type actual
+   | DE_TooManyValues => "too many values"
+   | DE_TooFewValues => "too few values"
+   | DE_LocalNameShadowing name => "local name shadowed: " ++ name
+   | DE_LeaveWithoutFunction => "leave without function"
+   | DE_LeftoverValuesInExpression => "leftover values in expression (use drop())"
+   | DE_SingleBooleanExpected => "single boolean expected"
+   | DE_SingleValueExpected => "single value expected"
+   | DE_BreakContinueDisallowed => "break and continue not allowed"
+   end.
+
+
+
+(*
+
+:= 
+
+(** A function is called with an argument of a unexpected type
+    or an initializer of a variable returns a value of a wrong type. *)
+ | DE_VarTypeMismatch
+(** There are two local variables (that includes inputs or outputs) with the same name. *)
+ | DE_LocalNameShadowing
+(** An expression has returned multiple values in the context in which only one was expected. *)
+ | DE_ExactlyOneValueExpected
+(** A function is declared with the same name as one of the built-in functions. *)
+ | DE_BuiltinFunctionShadowing
+(** A function is declared with the same name as a function visible from its location. *)
+ | DE_LocalFunctionShadowing
+ | DE_CannotResolveFunction
+ | DE_CannotResolveVariable
+ | DE_InternalErrorOutputNotFound
+ | DE_UnexpectedBreak
+ | DE_UnexpectedContinue. *)
