L50/Expr.v
@@ -1,0 +1,85 @@
+From Coq Require Import String Arith.
+
+From Vyper Require Import Config Map.
+From Vyper.L10 Require Import Base.
+From Vyper.L50 Require Import Types AST Builtins.
+
+(**
+    Prepend a newly computed result to a tuple of computed values.
+    The newly computed result must contain exactly one value,
+    otherwise [DE_ExactlyOneValueExpected] will be "thrown".
+ *)
+Definition cons_eval_results {C: VyperConfig}
+                             (head: option (expr_result (list dynamic_value)))
+                             (tail: list dynamic_value)
+: option (expr_result (list dynamic_value))
+:= match head with
+   | None | Some (ExprAbort _) => head
+   | Some (ExprSuccess h_values) =>
+      match h_values with
+      | (v :: nil)%list => Some (ExprSuccess (v :: tail)%list)
+      | _ => Some (expr_error "exactly one value expected")
+      end
+   end.
+
+Fixpoint interpret_expr {C: VyperConfig}
+                        (builtins: string -> option yul_builtin)
+                        (funs: string -> option fun_decl)
+                        (do_call: fun_decl -> world_state -> list dynamic_value ->
+                                    world_state * option (expr_result (list dynamic_value)))
+                        (world: world_state)
+                        (loc: string_map dynamic_value)
+                        (e: expr)
+{struct e}
+: world_state * option (expr_result (list dynamic_value))
+:= let fix interpret_expr_list (world: world_state)
+                               (loc: string_map dynamic_value)
+                               (args: list expr)
+    {struct args}
+    : world_state * option (expr_result (list dynamic_value))
+    := match args with
+       | nil => (world, Some (ExprSuccess nil))
+       | cons head tail =>
+           (* Arguments are evaluated right-to-left. *)
+           let tail_result := interpret_expr_list world loc tail
+           in match tail_result with
+              | (_, Some (ExprAbort _)) | (_, None) => tail_result
+              | (world', Some (ExprSuccess tail_values)) =>
+                 let '(world'', head_result) := interpret_expr builtins funs do_call
+                                                               world' loc head
+                  in (world'', cons_eval_results head_result tail_values)
+              end
+   end in
+   match e with
+   | Const type val => (world, Some (ExprSuccess (existT _ type val :: nil)%list))
+   | LocVar id =>
+          let _ := string_map_impl in
+          match Map.lookup loc id with
+          | None => (world, Some (expr_error "cannot resolve variable"))
+          | Some value =>
+              (world, Some (ExprSuccess (value :: nil)%list))
+          end
+   | FunCall name args =>
+      match builtins name with
+      | Some b =>
+          match funs name with
+          | Some f => (world, Some (expr_error "a function shadows a builtin"))
+          | None => (* call builtin *)
+             match interpret_expr_list world loc args with
+             | (world', Some (ExprSuccess arg_values)) =>
+                  let '(world'', result) := call_builtin b world' arg_values in
+                  (world'', Some result)
+             | _ as result => result
+             end
+          end
+      | None =>
+          match funs name with
+          | None => (world, Some (expr_error "can't resolve function name"))
+          | Some f => (* call function *)
+               match interpret_expr_list world loc args with
+               | (world', Some (ExprSuccess arg_values)) => do_call f world' arg_values
+               | _ as result => result
+               end
+          end
+      end
+  end.
