L50/LocalVars.v
@@ -1,0 +1,111 @@
+From Coq Require Import String Arith.
+
+From Vyper Require Import Config Map.
+From Vyper.L10 Require Import Base.
+From Vyper.L50 Require Import Types AST Builtins DynError.
+
+Local Open Scope list_scope.
+
+(** Lookup all the names in the variable map and check types. 
+    The names need not be distinct.
+ *)
+Fixpoint get_vars_by_typenames {C: VyperConfig}
+                               (typenames: list typename)
+                               (vars: string_map dynamic_value)
+: dynamic_error + list dynamic_value
+:= match typenames with
+   | nil => inr nil
+   | (type, name) :: rest =>
+       match map_lookup vars name as z return (_ = z -> _) with
+       | None => fun _ => inl (DE_CannotResolveLocalVariable name)
+       | Some value => fun found =>
+           let t := projT1 value in 
+           if yul_type_eq_dec type t
+             then match get_vars_by_typenames rest vars with
+                  | inl err => inl err
+                  | inr rest_results => inr (value :: rest_results)
+                  end
+             else inl (DE_TypeMismatch type t)
+       end eq_refl
+   end.
+
+(** Bind several variables. This happens to the function arguments right after a call
+    and also in a variable declaration with initializer.
+    The names must be distinct because shadowing is not allowed.
+ *)
+Fixpoint bind_vars_to_values {C: VyperConfig}
+                             (vars: list typename)
+                             (init: list dynamic_value)
+                             (loc: string_map dynamic_value)
+: dynamic_error + string_map dynamic_value
+:= match vars with
+   | nil =>
+      match init with
+      | nil => inr loc
+      | _ => inl DE_TooManyValues
+      end
+   | (vtype, vname) :: vtail =>
+      match init with
+      | nil => inl DE_TooFewValues
+      | (existT _ itype ivalue as ihead) :: itail =>
+          if yul_type_eq_dec vtype itype then
+            match map_lookup loc vname with
+            | Some _ => inl (DE_LocalNameShadowing vname)
+            | None => bind_vars_to_values vtail itail (map_insert loc vname ihead)
+            end
+          else inl (DE_TypeMismatch vtype itype)
+      end
+   end.
+
+(** Bind several variables to zeros. 
+    This happens to the function outputs right after a call
+    and also in a variable declaration without initializer.
+    The names must be distinct because shadowing is not allowed.
+*)
+Fixpoint bind_vars_to_zeros {C: VyperConfig}
+                            (vars: list typename)
+                            (loc: string_map dynamic_value)
+: dynamic_error + string_map dynamic_value
+:= match vars with
+   | nil => inr loc
+   | (vtype, vname) :: vtail =>
+        match map_lookup loc vname with
+        | Some _ => inl (DE_LocalNameShadowing vname)
+        | None => bind_vars_to_zeros vtail (map_insert loc vname (existT _ vtype (zero_value vtype)))
+        end
+   end.
+
+(** Rebind several variables. This happens in assignments. *)
+Fixpoint rebind_vars_to_values {C: VyperConfig}
+                               (vars: list string)
+                               (rhs: list dynamic_value)
+                               (loc: string_map dynamic_value)
+: dynamic_error + string_map dynamic_value
+:= match vars with
+   | nil =>
+      match rhs with
+      | nil => inr loc
+      | _ => inl DE_TooManyValues
+      end
+   | vname :: vtail =>
+      match rhs with
+      | nil => inl DE_TooFewValues
+      | (existT _ rtype rvalue as rhead) :: rtail =>
+            match map_lookup loc vname with
+            | Some (existT _ vtype _) =>
+                if yul_type_eq_dec vtype rtype
+                  then rebind_vars_to_values vtail rtail (map_insert loc vname rhead)
+                  else inl (DE_TypeMismatch rtype vtype)
+            | None => inl (DE_CannotResolveLocalVariable vname)
+            end
+      end
+   end.
+
+Fixpoint unbind_vars {C: VyperConfig}
+                     (vars: list typename)
+                     (loc: string_map dynamic_value)
+: string_map dynamic_value
+:= match vars with
+   | nil => loc
+   | h :: t => unbind_vars t (map_remove loc (snd h))
+   end.
