L50/Stmt.v
@@ -1,0 +1,220 @@
+From Coq Require Import String Arith ZArith.
+
+From Vyper Require Import Config Map.
+From Vyper.L10 Require Import Base.
+From Vyper.L50 Require Import Types AST Builtins Expr LocalVars DynError.
+
+Local Open Scope list_scope.
+
+Local Lemma var_decl_helper {C: VyperConfig} {s: stmt} {vars init}
+                            (NotVarDecl: is_var_decl s = false)
+                            (E: s = VarDecl vars init):
+  False.
+Proof.
+now subst.
+Qed.
+
+(* This is needed for the [preproc] argument in interpret_block which is needed for for-loop inits blocks. *)
+Definition nop {C: VyperConfig} (world: world_state) (loc: string_map dynamic_value)
+: world_state * string_map dynamic_value * option (stmt_result (list dynamic_value))
+:= (world, loc, Some StmtSuccess).
+
+Fixpoint interpret_stmt {C: VyperConfig}
+                        (max_loop_iterations: nat)
+                        (builtins: string -> option yul_builtin)
+                        (funs: string -> option fun_decl)
+                        (this_fun_decl: option fun_decl)
+                        (do_call: fun_decl -> world_state -> list dynamic_value ->
+                                    world_state * option (expr_result (list dynamic_value)))
+                        (world: world_state)
+                        (loc: string_map dynamic_value)
+                        (s: stmt)
+                        (NotVarDecl: is_var_decl s = false)
+{struct s}
+: world_state * string_map dynamic_value * option (stmt_result (list dynamic_value))
+:= match s as s' return s = s' -> _ with
+   | Break => fun _ => (world, loc, Some (StmtAbort AbortBreak))
+   | Continue => fun _ => (world, loc, Some (StmtAbort AbortContinue))
+   | Leave => fun _ =>
+              match this_fun_decl with
+              | None => (world, loc, Some (stmt_error (string_of_dynamic_error DE_LeaveWithoutFunction)))
+              | Some f => match get_vars_by_typenames (fd_outputs f) loc with
+                          | inl err => (world, loc, Some (stmt_error (string_of_dynamic_error err)))
+                          | inr outputs => (world, loc, Some (StmtReturnFromFunction outputs))
+                          end
+              end
+   | BlockStmt b => fun _ => interpret_block max_loop_iterations
+                                             builtins funs this_fun_decl do_call
+                                             world loc nop b
+   | VarDecl _ _ => fun E => match var_decl_helper NotVarDecl E with end
+   | Assign names rhs => fun _ =>
+            match interpret_expr builtins funs do_call world loc rhs
+            with
+            | (world', Some (ExprSuccess values)) =>
+                match rebind_vars_to_values names values loc with
+                | inl err => (world', loc, Some (stmt_error (string_of_dynamic_error err)))
+                | inr loc' => (world', loc', Some StmtSuccess)
+                end
+            | (world', Some (ExprAbort ab)) => (world', loc, Some (StmtAbort ab))
+            | (world', None) => (world', loc, None)
+            end
+   | If cond yes => fun _ =>
+           match interpret_expr builtins funs do_call world loc cond
+           with
+           | (world', Some (ExprSuccess (existT _ BoolType (BoolValue _ b _) :: nil))) =>
+               if b
+                 then interpret_block max_loop_iterations
+                                      builtins funs this_fun_decl do_call
+                                      world loc nop yes
+                 else (world', loc, Some StmtSuccess)
+           | (world', Some (ExprSuccess _)) =>
+                (world', loc, Some (stmt_error (string_of_dynamic_error DE_SingleBooleanExpected)))
+           | (world', Some (ExprAbort ab)) => (world', loc, Some (StmtAbort ab))
+           | (world', None) => (world', loc, None)
+           end
+   | Expr e => fun _ =>
+               match interpret_expr builtins funs do_call world loc e
+               with
+               | (world', Some (ExprSuccess nil)) => (world', loc, Some StmtSuccess)
+               | (world', Some (ExprSuccess _)) =>
+                    (world', loc, Some (stmt_error (string_of_dynamic_error DE_LeftoverValuesInExpression)))
+               | (world', Some (ExprAbort ab)) => (world', loc, Some (StmtAbort ab))
+               | (world', None) => (world', loc, None)
+               end
+   | Switch e cases default => fun _ =>
+       let (world', result) := interpret_expr builtins funs do_call world loc e
+       in match result with
+          | Some (ExprSuccess (existT _ value_type value :: nil)) =>
+              (fix dispatch (l: list case)
+               : world_state * string_map dynamic_value * option (stmt_result (list dynamic_value))
+               := match l with
+                  | (Case guard_type guard body) :: tail =>
+                      if yul_type_eq_dec value_type guard_type
+                        then if (Z_of_uint256 (uint256_of_yul_value value)
+                                  =?
+                                 Z_of_uint256 (uint256_of_yul_value guard))%Z
+                                then interpret_block max_loop_iterations
+                                                     builtins funs this_fun_decl do_call
+                                                     world loc nop body
+                                else dispatch tail
+                        else (world', loc, Some (stmt_error (string_of_dynamic_error
+                                                              (DE_TypeMismatch guard_type value_type))))
+                  | nil =>
+                           match default with
+                           | Some body =>
+                                interpret_block max_loop_iterations
+                                                builtins funs this_fun_decl do_call
+                                                world loc nop body
+                           | None => (world', loc, Some StmtSuccess)
+                           end
+                  end) cases
+          | Some (ExprSuccess _) =>
+              (world', loc, Some (stmt_error (string_of_dynamic_error DE_SingleValueExpected)))
+          | Some (ExprAbort ab) => (world', loc, Some (StmtAbort ab))
+          | None => (world', loc, None)
+          end
+   | For init cond after body => fun _ =>
+        let fix iterate (count: nat) (world: world_state) (loc: string_map dynamic_value)
+            : world_state * string_map dynamic_value * option (stmt_result (list dynamic_value))
+            := match count with
+               | O => (world, loc, None)
+               | S count' =>
+                   match interpret_expr builtins funs do_call world loc cond
+                   with
+                   | (world', Some (ExprSuccess (existT _ BoolType (BoolValue _ b _) :: nil))) =>
+                       if b
+                         then match interpret_block max_loop_iterations
+                                                    builtins funs this_fun_decl do_call
+                                                    world' loc nop body
+                              with
+                              | (world'', loc', Some (StmtAbort AbortBreak)) =>
+                                  (world'', loc', Some StmtSuccess)
+                              | (world'', loc', Some (StmtAbort AbortContinue))
+                              | (world'', loc', Some StmtSuccess) =>
+                                  match interpret_block max_loop_iterations
+                                                        builtins funs this_fun_decl do_call
+                                                        world'' loc' nop after
+                                  with
+                                  | (world''', loc'', Some (StmtAbort AbortBreak))
+                                  | (world''', loc'', Some (StmtAbort AbortContinue)) =>
+                                      (world''', loc'', Some (stmt_error
+                                                          (string_of_dynamic_error
+                                                            DE_BreakContinueDisallowed)))
+                                  | (world''', loc'', Some StmtSuccess) =>
+                                      iterate count' world''' loc''
+                                  | x => x
+                                  end
+                              | x => x
+                              end
+                         else (world', loc, Some StmtSuccess)
+                   | (world', Some (ExprSuccess _)) =>
+                        (world', loc, Some (stmt_error (string_of_dynamic_error DE_SingleBooleanExpected)))
+                   | (world', Some (ExprAbort ab)) => (world', loc, Some (StmtAbort ab))
+                   | (world', None) => (world', loc, None)
+                   end
+               end
+        in match interpret_block max_loop_iterations
+                                 builtins funs this_fun_decl do_call
+                                 world loc (iterate max_loop_iterations) init
+           with
+           | (world', loc', Some (StmtAbort AbortBreak))
+           | (world', loc', Some (StmtAbort AbortContinue)) =>
+               (world', loc', Some (stmt_error (string_of_dynamic_error DE_BreakContinueDisallowed)))
+           | x => x
+           end
+   end eq_refl
+with interpret_block {C: VyperConfig}
+                     (max_loop_iterations: nat)
+                     (builtins: string -> option yul_builtin)
+                     (funs: string -> option fun_decl)
+                     (this_fun_decl: option fun_decl)
+                     (do_call: fun_decl -> world_state -> list dynamic_value ->
+                                 world_state * option (expr_result (list dynamic_value)))
+                     (world: world_state)
+                     (loc: string_map dynamic_value)
+                     (postproc: world_state -> string_map dynamic_value ->
+                                world_state * string_map dynamic_value * option (stmt_result (list dynamic_value)))
+                     (b: block)
+: world_state * string_map dynamic_value * option (stmt_result (list dynamic_value))
+:= let fix interpret_stmt_list (world: world_state)
+                               (loc: string_map dynamic_value)
+                               (stmts: list stmt)
+        {struct stmts}
+        : world_state * string_map dynamic_value * option (stmt_result (list dynamic_value))
+        := match stmts as stmts' return stmts = stmts' -> _ with
+           | nil => fun _ => postproc world loc
+           | h :: t => fun E =>
+              (if is_var_decl h as h_is_var_decl return _ = h_is_var_decl -> _
+                 then fun Evar =>
+                   match var_decl_unpack h Evar with
+                   | (names, Some init) =>
+                        match interpret_expr builtins funs do_call world loc init
+                        with
+                        | (world', Some (ExprSuccess values)) =>
+                            match bind_vars_to_values names values loc with
+                            | inl err => (world', loc, Some (stmt_error (string_of_dynamic_error err)))
+                            | inr loc' =>
+                                let '(world'', loc'', result) := interpret_stmt_list world' loc' t in
+                                (world'', unbind_vars names loc'', result)
+                            end
+                        | (world', Some (ExprAbort ab)) => (world', loc, Some (StmtAbort ab))
+                        | (world', None) => (world', loc, None)
+                        end
+                   | (names, None) =>
+                       match bind_vars_to_zeros names loc with
+                       | inl err => (world, loc, Some (stmt_error (string_of_dynamic_error err)))
+                       | inr loc' =>
+                           let '(world', loc'', result) := interpret_stmt_list world loc' t in
+                           (world', unbind_vars names loc'', result)
+                       end
+                   end
+                 else fun Evar =>
+                   let '(world', loc', result) := interpret_stmt max_loop_iterations
+                                                                 builtins funs this_fun_decl do_call
+                                                                 world loc h Evar
+                   in match result with
+                      | Some StmtSuccess => interpret_stmt_list world' loc' t
+                      | _ => (world', loc', result)
+                      end) eq_refl
+           end eq_refl
+    in let '(Block stmts) := b in interpret_stmt_list world loc stmts.
