L50/Types.v
@@ -1,0 +1,332 @@
+From Coq Require Import ZArith Ascii String Eqdep_dec.
+From Vyper Require Import Config.
+
+Inductive int_size
+:= I8 | I32 | I64 | I128 | I256.
+
+Definition int_size_in_bits (i: int_size): Z
+:= match i with
+   | I8 => 8
+   | I32 => 32
+   | I64 => 64
+   | I128 => 128
+   | I256 => 256
+   end.
+
+Definition int_size_in_bytes (i: int_size): Z
+:= match i with
+   | I8 => 1
+   | I32 => 4
+   | I64 => 8
+   | I128 => 16
+   | I256 => 32
+   end.
+
+Lemma int_size_ok (i: int_size):
+  int_size_in_bits i = (8 * int_size_in_bytes i)%Z.
+Proof.
+  destruct i; trivial. 
+Qed.
+
+Definition string_of_int_size (i: int_size): string
+:= match i with
+   | I8 => "8"
+   | I32 => "32"
+   | I64 => "64"
+   | I128 => "128"
+   | I256 => "256"
+   end.
+
+Definition int_size_of_string (s: string): option int_size
+:= match s with
+   | "8"%string => Some I8
+   | "32"%string => Some I32
+   | "64"%string => Some I64
+   | "128"%string => Some I128
+   | "256"%string => Some I256
+   | _ => None
+   end.
+
+Lemma int_size_of_string_of_int_size (i: int_size):
+  int_size_of_string (string_of_int_size i) = Some i.
+Proof.
+now destruct i.
+Qed.
+
+Definition uint_max (i: int_size) := (2 ^ int_size_in_bits i - 1)%Z.
+Definition sint_max (i: int_size) := (2 ^ (int_size_in_bits i - 1) - 1)%Z.
+Definition sint_min (i: int_size) := (- 2 ^ (int_size_in_bits i - 1))%Z.
+
+Example uint_max_byte: uint_max I8 = 255%Z.    Proof. trivial. Qed.
+Example sint_min_byte: sint_min I8 = (-128)%Z. Proof. trivial. Qed.
+Example sint_max_byte: sint_max I8 = 127%Z.    Proof. trivial. Qed.
+
+Inductive yul_type
+:= BoolType
+ | IntType (size: int_size) (signed: bool).
+
+Lemma yul_type_eq_dec (a b: yul_type)
+: {a = b} + {a <> b}.
+Proof.
+repeat decide equality.
+Defined.
+
+Definition U8 := IntType I8 false.
+Definition S8 := IntType I8 true.
+Definition U32 := IntType I32 false.
+Definition S32 := IntType I32 true.
+Definition U64 := IntType I64 false.
+Definition S64 := IntType I64 true.
+Definition U128 := IntType I128 false.
+Definition S128 := IntType I128 true.
+Definition U256 := IntType I256 false.
+Definition S256 := IntType I256 true.
+
+Definition uint256_to_Z_as_signed {C: VyperConfig} (n: uint256)
+: Z
+:= let z := Z_of_uint256 n in
+   if Z.testbit z 255%Z
+     then z - 2 ^ 256
+     else z.
+
+Inductive yul_value {C: VyperConfig} (t: yul_type)
+:= NumberValue (value: uint256)
+               (ok: match t with
+                    | BoolType => false
+                    | IntType size true  => let x := uint256_to_Z_as_signed value in
+                                            andb (sint_min size <=? x)%Z (x <=? sint_max size)%Z
+                    | IntType size false => let x := Z_of_uint256 value in
+                                            andb (0 <=? x)%Z (x <=? uint_max size)%Z
+                    end = true)
+ | BoolValue (b: bool)
+             (ok:  match t with
+                   | BoolType => true
+                   | _ => false
+                   end = true).
+
+Definition yul_true  {C: VyperConfig} := BoolValue BoolType true eq_refl.
+Definition yul_false {C: VyperConfig} := BoolValue BoolType false eq_refl.
+
+Lemma yul_uint256_helper {C: VyperConfig} (value: uint256):
+  ((0 <=? Z_of_uint256 value)%Z && (Z_of_uint256 value <=? uint_max I256)%Z)%bool = true.
+Proof.
+assert (R := uint256_range value).
+apply andb_true_intro. split.
+now rewrite Z.leb_le.
+unfold uint_max. unfold int_size_in_bits.
+rewrite Z.leb_le.
+apply Zsucc_le_reg.
+replace (Z.succ (2 ^ 256 - 1))%Z with (2 ^ 256)%Z by trivial.
+now apply Zlt_le_succ.
+Qed.
+
+Definition yul_uint256 {C: VyperConfig} (value: uint256)
+: yul_value U256
+:= NumberValue U256 value (yul_uint256_helper value).
+
+Definition dynamic_value {C: VyperConfig} := { t: yul_type & yul_value t }.
+
+Definition uint256_of_yul_value {C: VyperConfig} {t: yul_type} (y: yul_value t)
+: uint256
+:= match y with
+   | NumberValue _ value _ => value
+   | BoolValue _ true  _ => one256
+   | BoolValue _ false _ => zero256
+   end.
+
+Local Lemma uint256_to_yul_value_helper_bool {C: VyperConfig} {t: yul_type} (T: t = BoolType):
+   match t with
+   | BoolType => true
+   | IntType _ _ => false
+   end = true.
+Proof.
+now subst.
+Qed.
+
+Local Lemma uint256_to_yul_value_helper_sint {C: VyperConfig} {t: yul_type} {u : uint256}
+                                             {size: int_size} (T: t = IntType size true)
+                                             (E: let x := uint256_to_Z_as_signed u in
+                                                  ((sint_min size <=? x)%Z &&
+                                                    (x <=? sint_max size)%Z)%bool = true):
+   match t with
+   | BoolType => false
+   | IntType size true =>
+       let x := uint256_to_Z_as_signed u in ((sint_min size <=? x)%Z && (x <=? sint_max size)%Z)%bool
+   | IntType size false => let x := Z_of_uint256 u in ((0 <=? x)%Z && (x <=? uint_max size)%Z)%bool
+   end = true.
+Proof.
+now subst.
+Qed.
+
+Local Lemma uint256_to_yul_value_helper_uint {C: VyperConfig} {t: yul_type} {u : uint256}
+                                             {size: int_size} (T: t = IntType size false)
+                                             (E: let x := Z_of_uint256 u in
+                                                  ((0 <=? x)%Z && (x <=? uint_max size)%Z)%bool = true):
+   match t with
+   | BoolType => false
+   | IntType size true =>
+       let x := uint256_to_Z_as_signed u in ((sint_min size <=? x)%Z && (x <=? sint_max size)%Z)%bool
+   | IntType size false => let x := Z_of_uint256 u in ((0 <=? x)%Z && (x <=? uint_max size)%Z)%bool
+   end = true.
+Proof.
+now subst.
+Qed.
+
+Definition yul_value_of_uint256 {C: VyperConfig} (u: uint256) (t: yul_type)
+: option (yul_value t)
+:= match t as t' return t = t' -> _ with
+   | BoolType => fun T =>
+                 match Z_of_uint256 u with
+                 | 0%Z => Some (BoolValue t false (uint256_to_yul_value_helper_bool T))
+                 | 1%Z => Some (BoolValue t true (uint256_to_yul_value_helper_bool T))
+                 | _ => None
+                 end
+   | IntType size true => fun T =>
+                          let x := uint256_to_Z_as_signed u in
+                          (if andb (sint_min size <=? x)%Z (x <=? sint_max size)%Z as c
+                           return _ = c -> _
+                             then fun E => Some (NumberValue t u (uint256_to_yul_value_helper_sint T E))
+                             else fun _ => None) eq_refl
+   | IntType size false => fun T =>
+                           let x := Z_of_uint256 u in
+                           (if andb (0 <=? x)%Z (x <=? uint_max size)%Z as c return _ = c -> _
+                              then fun E => Some (NumberValue t u (uint256_to_yul_value_helper_uint T E))
+                              else fun _ => None) eq_refl
+   end eq_refl.
+
+Lemma yul_value_of_uint256_of_yul_value {C: VyperConfig} (t: yul_type) (v: yul_value t):
+  yul_value_of_uint256 (uint256_of_yul_value v) t = Some v.
+Proof.
+destruct t; cbn; destruct v; try discriminate.
+{
+  destruct b; cbn; [unfold one256 | unfold zero256];
+     rewrite uint256_ok; cbn; repeat f_equal; apply eq_proofs_unicity;
+     decide equality.
+}
+destruct signed; cbn in *.
+{
+  (* signed *)
+  remember (fun E =>
+             Some (NumberValue (IntType size true) value (uint256_to_yul_value_helper_sint eq_refl E)))
+    as good_branch.
+  enough (Q: forall E, good_branch E = Some (NumberValue (IntType size true) value ok)).
+  {
+    clear Heqgood_branch.
+    revert good_branch Q.
+    assert (ok' := ok).
+    now rewrite ok'.
+  }
+  intros.
+  subst. repeat f_equal.
+  apply eq_proofs_unicity; decide equality.
+}
+(* unsigned *)
+remember (fun E =>
+           Some (NumberValue (IntType size false) value (uint256_to_yul_value_helper_uint eq_refl E)))
+  as good_branch.
+enough (Q: forall E, good_branch E = Some (NumberValue (IntType size false) value ok)).
+{
+  clear Heqgood_branch.
+  revert good_branch Q.
+  assert (ok' := ok).
+  now rewrite ok'.
+}
+intros.
+subst. repeat f_equal.
+apply eq_proofs_unicity; decide equality.
+Qed.
+
+Definition uint256_of_dynamic_value {C: VyperConfig} (d: dynamic_value)
+: uint256
+:= let '(existT _ _ v) := d in
+   uint256_of_yul_value v.
+
+Lemma bool_eq_via_uint256 {C: VyperConfig}
+                          (a b: bool)
+                          (E: (if a then one256 else zero256)
+                               =
+                              (if b then one256 else zero256)):
+  a = b.
+Proof.
+assert (E': Z_of_uint256 (if a then one256 else zero256) = Z_of_uint256 (if b then one256 else zero256))
+  by now rewrite E.
+unfold one256 in E'. unfold zero256 in E'.
+destruct a, b; repeat rewrite uint256_ok in E'; now try discriminate.
+Qed.
+
+Lemma yul_value_eq_via_uint256 {C: VyperConfig}
+                               (t: yul_type)
+                               (a b: yul_value t)
+                               (E: uint256_of_yul_value a = uint256_of_yul_value b):
+  a = b.
+Proof.
+unfold uint256_of_yul_value in E.
+destruct a, b, t; try discriminate; [| apply bool_eq_via_uint256 in E ];
+  subst; f_equal; apply Eqdep_dec.eq_proofs_unicity; decide equality.
+Qed.
+
+Definition string_of_type (t: yul_type)
+:= match t with
+   | BoolType => "bool"%string
+   | IntType size signed => String (if signed then "s"%char else "u"%char) (string_of_int_size size)
+   end.
+
+Example string_of_u256: string_of_type U256 = "u256"%string. Proof. trivial. Qed.
+
+Definition type_of_string (s: string)
+: option yul_type
+:= match s with
+   | String "s"%char size =>
+        match int_size_of_string size with
+        | Some s => Some (IntType s true)
+        | None => None
+        end
+   | String "u"%char size =>
+        match int_size_of_string size with
+        | Some s => Some (IntType s false)
+        | None => None
+        end
+   | "bool"%string => Some BoolType
+   | _ => None
+   end.
+
+Lemma type_of_string_of_type (t: yul_type):
+  type_of_string (string_of_type t) = Some t.
+Proof.
+destruct t as [|size]. { trivial. }
+now destruct size, signed.
+Qed.
+
+
+Local Lemma int_zero_value_helper {C: VyperConfig} (size: int_size) (signed: bool):
+   match IntType size signed with
+   | BoolType => false
+   | IntType size true =>
+       let x := uint256_to_Z_as_signed zero256 in
+       ((sint_min size <=? x)%Z && (x <=? sint_max size)%Z)%bool
+   | IntType size false =>
+       let x := Z_of_uint256 zero256 in ((0 <=? x)%Z && (x <=? uint_max size)%Z)%bool
+   end = true.
+Proof.
+cbn. unfold zero256. unfold uint256_to_Z_as_signed.
+rewrite uint256_ok. cbn.
+now destruct signed, size.
+Qed.
+
+Definition int_zero_value {C: VyperConfig} (size: int_size) (signed: bool)
+: yul_value (IntType size signed)
+:= NumberValue (IntType size signed) zero256 (int_zero_value_helper size signed).
+
+
+Definition zero_value {C: VyperConfig} (t: yul_type)
+: yul_value t
+:= match t with
+   | BoolType => yul_false
+   | IntType size signed => int_zero_value size signed
+   end.
+
+Lemma zero_value_ok {C: VyperConfig} (t: yul_type):
+  Z_of_uint256 (uint256_of_yul_value (zero_value t)) = 0%Z.
+Proof.
+destruct t; cbn; unfold zero256; rewrite uint256_ok; trivial.
+Qed.
