ProtoAST.v
@@ -1,0 +1,10 @@
+From Coq Require Import String.
+
+(** A prototype of a builtin function.
+  This is just an AST: types are just strings.
+ *)
+Record proto_ast := {
+  proto_name: string;
+  proto_inputs: list string;
+  proto_outputs: list string;
+}.
